read32, write32 bounded int32

src/lowparse/LowParse.Low.BoundedInt.fst
@@ -82,6 +82,78 @@ let serialize32_bounded_integer_4 () =
   E.n_to_be_4 _ _ (E.u32 ()) v out pos;
   4ul
 
+inline_for_extraction
+let write_bounded_int32'
+  (min32: U32.t)
+  (max32: U32.t { 0 < U32.v max32 /\ U32.v min32 <= U32.v max32 /\ U32.v max32 < 4294967296 })
+  (sz: nat { sz == log256' (U32.v max32) })
+: Tot (leaf_writer_strong (serialize_bounded_int32 (U32.v min32) (U32.v max32)))
+= [@inline_let]
+  let min = U32.v min32 in
+  [@inline_let]
+  let max = U32.v max32 in
+  write_synth
+    (write_filter
+      (write_bounded_integer sz)
+      (in_bounds min max))
+    (fun x -> (x <: bounded_int32 min max))
+    (fun x -> x)
+    (fun x -> x)
+    ()
+
+let write_bounded_int32_1
+  min32 max32
+= write_bounded_int32' min32 max32 1
+
+let write_bounded_int32_2
+  min32 max32
+= write_bounded_int32' min32 max32 2
+
+let write_bounded_int32_3
+  min32 max32
+= write_bounded_int32' min32 max32 3
+
+let write_bounded_int32_4
+  min32 max32
+= write_bounded_int32' min32 max32 4
+
+inline_for_extraction
+let read_bounded_int32'
+  (min32: U32.t)
+  (max32: U32.t { 0 < U32.v max32 /\ U32.v min32 <= U32.v max32 /\ U32.v max32 < 4294967296 })
+  (sz: nat { sz == log256' (U32.v max32) })
+: Tot (leaf_reader (parse_bounded_int32 (U32.v min32) (U32.v max32)))
+= 
+  [@inline_let]
+  let min = U32.v min32 in
+  [@inline_let]
+  let max = U32.v max32 in
+  read_synth
+    (parse_filter (parse_bounded_integer sz) (in_bounds min max))
+    (fun x -> (x <: bounded_int32 min max))
+    (fun x -> x)
+    (read_filter
+      (read_bounded_integer sz)
+      (in_bounds min max))
+    ()
+
+let read_bounded_int32_1
+  min32 max32
+= read_bounded_int32' min32 max32 1
+
+let read_bounded_int32_2
+  min32 max32
+= read_bounded_int32' min32 max32 2
+
+let read_bounded_int32_3
+  min32 max32
+= read_bounded_int32' min32 max32 3
+
+let read_bounded_int32_4
+  min32 max32
+= read_bounded_int32' min32 max32 4
+
+
 let read_bounded_integer_le_1 =
   [@inline_let] let _ = bounded_integer_of_le_injective 1 in
   make_total_constant_size_reader 1 1ul #(bounded_integer 1) (bounded_integer_of_le 1) () (fun #rrel #rel b pos ->
